Veritas.Merkle.fsti
@@ -1,31 +1,9 @@
 module Veritas.Merkle
 
 open FStar.BitVector
+open Veritas.BinTree
 open Veritas.Memory
-
-(* Merkle address is simply a bin_tree_node of bounded depth *)
-type merkle_addr = n:bin_tree_node{depth n <= addr_size}
-
-(* Depth of a merkle node *)
-let merkle_depth (a:merkle_addr): Tot (i:nat {i <= addr_size}) = depth a
-
-(* Height of a merkle node *)
-let merkle_height (a:merkle_addr): Tot (i:nat {i <= addr_size}) = addr_size - merkle_depth a
-
-(* Merkle tree root *)
-let merkle_root:merkle_addr = Root
-
-(* Is this a merkle root *)
-let is_merkle_root (a:merkle_addr): Tot bool = (Root? a)
-
-(* Is this a leaf node *)
-let is_merkle_leaf (a:merkle_addr): Tot bool = merkle_height a = 0
-
-(* Helper refinement types of merkle addresses *)
-let merkle_leaf_addr = a:merkle_addr{is_merkle_leaf a}
-let merkle_root_addr = a:merkle_addr{is_merkle_root a}
-let merkle_non_leaf_addr = a:merkle_addr{~(is_merkle_leaf a)}
-let merkle_non_root_addr = a:merkle_addr{~(is_merkle_root a)}
+open Veritas.MerkleAddr
 
 (* Size of a hash value *)
 let hash_size = 256
@@ -56,29 +34,6 @@ type hash_collision =
                hash_collision
 
 (*
- * We want to use Merkle tree ideas to verify memory rw-consistency, where
- * memory is addressed locations of a 256-bit address space. To do that we
- * map (data) addresses to leaf nodes of the merkle tree. The leaf node 
- * for a 256-bit address is obtained by traversing the tree from the root 
- * taking a left child for a 0 bit and right child for a 1 bit
- *)
-
-val addr_to_merkle_leaf (a:addr): Tot merkle_leaf_addr
-
-(* Inverse of addr_to_merkle_leaf *)
-val merkle_leaf_to_addr (ma:merkle_leaf_addr): Tot (a:addr{addr_to_merkle_leaf a = ma})
-
-val lemma_addr_merkle_inv (a:addr):
-  Lemma (merkle_leaf_to_addr (addr_to_merkle_leaf a) = a)
-
-val lemma_merkle_equal_implies_addr_equal (a1:addr) (a2:addr):
-  Lemma (requires (addr_to_merkle_leaf a1 = addr_to_merkle_leaf a2))
-        (ensures (a1 = a2))
-
-val lemma_addr_equal_implies_merkle_equal (m1:merkle_leaf_addr) (m2:merkle_leaf_addr):
-  Lemma (requires (merkle_leaf_to_addr m1 = merkle_leaf_to_addr m2))
-        (ensures (m1 = m2))
-(*
  * merklefn: compute the merkle tree value at each node
  * of the merkle tree
  *)
@@ -89,27 +44,3 @@ let rec merklefn (a:merkle_addr) (mem: memory): Tot (merkle_payload_of_addr a)
   else MkInternal (hashfn (merklefn (LeftChild a) mem))
                   (hashfn (merklefn (RightChild a) mem))
         
-type desc_hash = 
-  | Empty: desc_hash
-  | Desc: a:merkle_addr -> h:hash_value -> desc_hash
-
-type sp_merkle_payload = 
-  | SMkLeaf: value:payload -> sp_merkle_payload
-  | SMkInternal: left:desc_hash -> right:desc_hash -> sp_merkle_payload
-
-(* hash function maps a merkle payload to a hash value *)
-val hashfn_sp (m:sp_merkle_payload): Tot hash_value
-
-(* Inductive type for hash collisions *) 
-type hash_collision_sp = 
-  | SCollision: m1:sp_merkle_payload ->
-                m2:sp_merkle_payload { hashfn_sp m1 == hashfn_sp m2 /\ ~(m1 == m2) } ->
-               hash_collision_sp
-
-let is_sp_payload_of_addr (a:merkle_addr) (p:sp_merkle_payload): Tot bool =
-  if is_merkle_leaf a then SMkLeaf? p 
-  else SMkInternal? p
-
-(* merkle payload type conditioned on the address *)
-type sp_merkle_payload_of_addr (a:merkle_addr) = 
-  p:sp_merkle_payload{is_sp_payload_of_addr a p}
