Veritas.MerkleAddr.fst
@@ -1,0 +1,30 @@
+module Veritas.MerkleAddr
+
+open FStar.BitVector
+open Veritas.BinTree
+
+(* 
+ * map each 256 bit address in memory to a leaf node of the 
+ * merkle tree
+ *)
+let addr_to_merkle_leaf (a:addr): Tot merkle_leaf_addr = 
+  bv_to_bin_tree_node a
+
+(* Inverse of addr_to_merkle_leaf *)
+let merkle_leaf_to_addr (ma:merkle_leaf_addr): Tot (a:addr{addr_to_merkle_leaf a = ma}) =
+  bin_tree_to_bv_consistent ma; bin_tree_node_to_bv ma
+
+let lemma_addr_merkle_inv (a:addr):
+  Lemma (merkle_leaf_to_addr (addr_to_merkle_leaf a) = a) = 
+  bv_to_bin_tree_consistent a
+
+let lemma_merkle_equal_implies_addr_equal (a1:addr) (a2:addr):
+  Lemma (requires (addr_to_merkle_leaf a1 = addr_to_merkle_leaf a2))
+        (ensures (a1 = a2)) = 
+  lemma_addr_merkle_inv a1;
+  lemma_addr_merkle_inv a2
+
+let lemma_addr_equal_implies_merkle_equal (m1:merkle_leaf_addr) (m2:merkle_leaf_addr):
+  Lemma (requires (merkle_leaf_to_addr m1 = merkle_leaf_to_addr m2))
+        (ensures (m1 = m2)) = ()
+
