Veritas.MerkleAddr.fsti
@@ -1,0 +1,44 @@
+module Veritas.MerkleAddr
+
+open Veritas.BinTree
+open Veritas.Memory
+
+(* Merkle address is simply a bin_tree_node of bounded depth *)
+type merkle_addr = n:bin_tree_node{depth n <= addr_size}
+
+(* Depth of a merkle node *)
+let merkle_depth (a:merkle_addr): Tot (i:nat {i <= addr_size}) = depth a
+
+(* Height of a merkle node *)
+let merkle_height (a:merkle_addr): Tot (i:nat {i <= addr_size}) = addr_size - merkle_depth a
+
+(* Merkle tree root *)
+let merkle_root:merkle_addr = Root
+
+(* Is this a merkle root *)
+let is_merkle_root (a:merkle_addr): Tot bool = (Root? a)
+
+(* Is this a leaf node *)
+let is_merkle_leaf (a:merkle_addr): Tot bool = merkle_height a = 0
+
+(* Helper refinement types of merkle addresses *)
+let merkle_leaf_addr = a:merkle_addr{is_merkle_leaf a}
+let merkle_root_addr = a:merkle_addr{is_merkle_root a}
+let merkle_non_leaf_addr = a:merkle_addr{~(is_merkle_leaf a)}
+let merkle_non_root_addr = a:merkle_addr{~(is_merkle_root a)}
+
+val addr_to_merkle_leaf (a:addr): Tot merkle_leaf_addr
+
+(* Inverse of addr_to_merkle_leaf *)
+val merkle_leaf_to_addr (ma:merkle_leaf_addr): Tot (a:addr{addr_to_merkle_leaf a = ma})
+
+val lemma_addr_merkle_inv (a:addr):
+  Lemma (merkle_leaf_to_addr (addr_to_merkle_leaf a) = a)
+
+val lemma_merkle_equal_implies_addr_equal (a1:addr) (a2:addr):
+  Lemma (requires (addr_to_merkle_leaf a1 = addr_to_merkle_leaf a2))
+        (ensures (a1 = a2))
+
+val lemma_addr_equal_implies_merkle_equal (m1:merkle_leaf_addr) (m2:merkle_leaf_addr):
+  Lemma (requires (merkle_leaf_to_addr m1 = merkle_leaf_to_addr m2))
+        (ensures (m1 = m2))
