Veritas.SparseMerkle.fsti
@@ -1,0 +1,37 @@
+module Veritas.SparseMerkle
+
+open FStar.BitVector
+open Veritas.BinTree
+open Veritas.MerkleAddr
+open Veritas.Memory
+
+(* Size of a hash value *)
+let hash_size = 256
+
+(* hash_value - bit vector of a specified size *)
+type hash_value = bv_t hash_size
+
+type desc_hash = 
+  | Empty: desc_hash
+  | Desc: a:merkle_addr -> h:hash_value -> desc_hash
+
+type merkle_payload = 
+  | SMkLeaf: value:payload -> merkle_payload
+  | SMkInternal: left:desc_hash -> right:desc_hash -> merkle_payload
+
+(* hash function maps a merkle payload to a hash value *)
+val hashfn (m:merkle_payload): Tot hash_value
+
+(* Inductive type for hash collisions *) 
+type hash_collision = 
+  | SCollision: m1:merkle_payload ->
+                m2:merkle_payload { hashfn m1 == hashfn m2 /\ ~(m1 == m2) } ->
+               hash_collision
+
+let is_payload_of_addr (a:merkle_addr) (p:merkle_payload): Tot bool =
+  if is_merkle_leaf a then SMkLeaf? p 
+  else SMkInternal? p
+
+(* merkle payload type conditioned on the address *)
+type merkle_payload_of_addr (a:merkle_addr) = 
+  p:merkle_payload{is_payload_of_addr a p}
